<?xml version="1.0"?>
<rdf:RDF xmlns="http://erlangen-crm.org/dimension#"
     xml:base="http://erlangen-crm.org/dimension"
     xmlns:owl="http://www.w3.org/2002/07/owl#"
     xmlns:rdf="http://www.w3.org/1999/02/22-rdf-syntax-ns#"
     xmlns:xml="http://www.w3.org/XML/1998/namespace"
     xmlns:xsd="http://www.w3.org/2001/XMLSchema#"
     xmlns:rdfs="http://www.w3.org/2000/01/rdf-schema#"
     xmlns:current="http://erlangen-crm.org/current/"
     xmlns:dimension="http://erlangen-crm.org/dimension#">
    <owl:Ontology rdf:about="http://erlangen-crm.org/dimension">
        <rdfs:comment>Dimension module extracted from CIDOC CRM Erlangen version 6.2.1</rdfs:comment>
        <owl:versionInfo xml:lang="en">Testing status</owl:versionInfo>
    </owl:Ontology>



    <!--
    ///////////////////////////////////////////////////////////////////////////////////////
    //
    // Object Properties
    //
    ///////////////////////////////////////////////////////////////////////////////////////
     -->




    <!-- http://erlangen-crm.org/current/P43_has_dimension -->

    <owl:ObjectProperty rdf:about="http://erlangen-crm.org/current/P43_has_dimension">
        <owl:inverseOf rdf:resource="http://erlangen-crm.org/current/P43i_is_dimension_of"/>
        <rdfs:domain rdf:resource="http://erlangen-crm.org/current/E77_Persistent_Item"/>
        <rdfs:range rdf:resource="http://erlangen-crm.org/current/E54_Dimension"/>
    </owl:ObjectProperty>



    <!-- http://erlangen-crm.org/current/P43i_is_dimension_of -->

    <owl:ObjectProperty rdf:about="http://erlangen-crm.org/current/P43i_is_dimension_of"/>



    <!-- http://erlangen-crm.org/dimension#hasQualitativeValue -->

    <owl:ObjectProperty rdf:about="http://erlangen-crm.org/dimension#hasQualitativeValue">
        <rdfs:domain rdf:resource="http://erlangen-crm.org/current/E54_Dimension"/>
        <rdfs:range rdf:resource="http://erlangen-crm.org/upper#QualitySpace"/>
    </owl:ObjectProperty>



    <!--
    ///////////////////////////////////////////////////////////////////////////////////////
    //
    // Data properties
    //
    ///////////////////////////////////////////////////////////////////////////////////////
     -->




    <!-- http://erlangen-crm.org/dimension#hasQuantitativeValue -->

    <owl:DatatypeProperty rdf:about="http://erlangen-crm.org/dimension#hasQuantitativeValue">
        <rdfs:comment xml:lang="en">This relation can be extended in order to model specific relations according to measurement units.

For example, hasLengthInCm, hasDiameterInMeter, etc.

This approach replaces the use of E58_Measurement_Unit</rdfs:comment>
    </owl:DatatypeProperty>



    <!--
    ///////////////////////////////////////////////////////////////////////////////////////
    //
    // Classes
    //
    ///////////////////////////////////////////////////////////////////////////////////////
     -->




    <!-- http://erlangen-crm.org/current/E54_Dimension -->

    <owl:Class rdf:about="http://erlangen-crm.org/current/E54_Dimension">
        <rdfs:subClassOf>
            <owl:Restriction>
                <owl:onProperty rdf:resource="http://erlangen-crm.org/current/P43i_is_dimension_of"/>
                <owl:someValuesFrom rdf:resource="http://erlangen-crm.org/current/E77_Persistent_Item"/>
            </owl:Restriction>
        </rdfs:subClassOf>
        <rdfs:comment xml:lang="en">In the original version of CIDOC, dimensions characterizes things. Since the class E70 Thing has been now removed, dimensions are attached to persistent items. This also allows to model the dimensions of actors.</rdfs:comment>
    </owl:Class>



    <!-- http://erlangen-crm.org/current/E77_Persistent_Item -->

    <owl:Class rdf:about="http://erlangen-crm.org/current/E77_Persistent_Item"/>



    <!-- http://erlangen-crm.org/dimension#RGBColorSpace -->

    <owl:Class rdf:about="http://erlangen-crm.org/dimension#RGBColorSpace">
        <rdfs:subClassOf rdf:resource="http://erlangen-crm.org/upper#QualitySpace"/>
        <rdfs:comment xml:lang="en">This class is added only for sake of the example</rdfs:comment>
    </owl:Class>



    <!-- http://erlangen-crm.org/upper#QualitySpace -->

    <owl:Class rdf:about="http://erlangen-crm.org/upper#QualitySpace">
        <rdfs:comment xml:lang="en">Quality space should be specialized in order to capture specific quality spaces. For example, the RGBColorSpace can be used to capture colors according to the RGB quality space.

For examples based on a similar approach, the reader can refer to
https://nemo-ufes.github.io/gufo/</rdfs:comment>
    </owl:Class>



    <!--
    ///////////////////////////////////////////////////////////////////////////////////////
    //
    // Individuals
    //
    ///////////////////////////////////////////////////////////////////////////////////////
     -->




    <!-- http://erlangen-crm.org/dimension#red -->

    <owl:NamedIndividual rdf:about="http://erlangen-crm.org/dimension#red">
        <rdf:type rdf:resource="http://erlangen-crm.org/dimension#RGBColorSpace"/>
        <rdfs:comment>this individual is added only for the sake of the example</rdfs:comment>
    </owl:NamedIndividual>



    <!-- http://erlangen-crm.org/dimension#t-shirt_id1 -->

    <owl:NamedIndividual rdf:about="http://erlangen-crm.org/dimension#t-shirt_id1">
        <current:P43_has_dimension rdf:resource="http://erlangen-crm.org/dimension#tshirt_id1-color"/>
        <rdfs:comment>this individual is added only for the sake of the example</rdfs:comment>
    </owl:NamedIndividual>



    <!-- http://erlangen-crm.org/dimension#tshirt_id1-color -->

    <owl:NamedIndividual rdf:about="http://erlangen-crm.org/dimension#tshirt_id1-color">
        <hasQualitativeValue rdf:resource="http://erlangen-crm.org/dimension#red"/>
        <rdfs:comment>this individual is added only for the sake of the example</rdfs:comment>
    </owl:NamedIndividual>



    <!--
    ///////////////////////////////////////////////////////////////////////////////////////
    //
    // General axioms
    //
    ///////////////////////////////////////////////////////////////////////////////////////
     -->

    <rdf:Description>
        <rdf:type rdf:resource="http://www.w3.org/2002/07/owl#AllDisjointClasses"/>
        <owl:members rdf:parseType="Collection">
            <rdf:Description rdf:about="http://erlangen-crm.org/current/E54_Dimension"/>
            <rdf:Description rdf:about="http://erlangen-crm.org/current/E77_Persistent_Item"/>
            <rdf:Description rdf:about="http://erlangen-crm.org/upper#QualitySpace"/>
        </owl:members>
    </rdf:Description>
</rdf:RDF>



<!-- Generated by the OWL API (version 4.5.9.2019-02-01T07:24:44Z) https://github.com/owlcs/owlapi -->
